split away full-CBOR parser specs; implement raw CBOR parser

src/cbor/spec/CBOR.Spec.API.Type.fsti
@@ -14,7 +14,7 @@
    limitations under the License.
 *)
 
-module CBOR.Spec.Type
+module CBOR.Spec.API.Type
 include CBOR.Spec.Constants
 
 module U8 = FStar.UInt8
@@ -132,100 +132,3 @@ val unpack_pack: (c: cbor_case) -> Lemma
 val pack_unpack: (c: cbor) -> Lemma
   (ensures (pack (unpack c) == c))
   [SMTPat (unpack c)]
-
-(** Parsing *)
-
-val cbor_parse : (x: Seq.seq U8.t) -> Pure (option (cbor & nat))
-  (requires True)
-  (ensures (fun res -> match res with
-  | None -> True
-  | Some (_, n) -> n <= Seq.length x
-  ))
-
-val cbor_parse_prefix
-  (x y: Seq.seq U8.t)
-: Lemma
-  (requires (match cbor_parse x with
-  | Some (_, n) -> Seq.length y >= n /\ Seq.slice x 0 n == Seq.slice y 0 n
-  | _ -> False
-  ))
-  (ensures (
-    cbor_parse x == cbor_parse y
-  ))
-
-(** Deterministic parsing and serialization *)
-
-val cbor_det_serialize: (x: cbor) -> Tot (Seq.seq U8.t)
-
-val cbor_det_parse (x: Seq.seq U8.t) : Pure (option (cbor & nat))
-  (requires True)
-  (ensures (fun res -> match res with
-  | None -> True
-  | Some (y, n) -> n <= Seq.length x /\ cbor_parse x == res /\ cbor_det_serialize y == Seq.slice x 0 n // unique binary representation
-  ))
-
-let cbor_det_parse_inj
-  (x1 x2: Seq.seq U8.t)
-: Lemma
-  (requires (match cbor_det_parse x1, cbor_det_parse x2 with
-  | Some (y1, n1), Some (y2, n2) -> y1 == y2
-  | _ -> False
-  ))
-  (ensures (match cbor_det_parse x1, cbor_det_parse x2 with
-  | Some (y1, n1), Some (y2, n2) -> y1 == y2 /\ n1 == n2 /\ Seq.slice x1 0 n1 == Seq.slice x2 0 n2
-  | _ -> False
-  ))
-= let Some (y1, n1) = cbor_det_parse x1 in
-  let Some (y2, n2) = cbor_det_parse x2 in
-  assert (Seq.slice x1 0 n1 == Seq.slice x2 0 n2);
-  assert (Seq.length (Seq.slice x1 0 n1) == Seq.length (Seq.slice x2 0 n2))
-
-val cbor_det_parse_prefix
-  (x y: Seq.seq U8.t)
-: Lemma
-  (requires (match cbor_det_parse x with
-  | Some (_, n) -> Seq.length y >= n /\ Seq.slice x 0 n `Seq.equal` Seq.slice y 0 n
-  | _ -> False
-  ))
-  (ensures (
-    cbor_det_parse x == cbor_det_parse y
-  ))
-
-val cbor_det_serialize_parse (x: cbor) : Lemma
-  (let s = cbor_det_serialize x in
-    cbor_det_parse s == Some (x, Seq.length s)
-  )
-
-let cbor_det_serialize_parse'
-  (x: cbor)
-  (y: Seq.seq U8.t)
-: Lemma
-  (let s = cbor_det_serialize x in
-    cbor_det_parse (s `Seq.append` y) == Some (x, Seq.length s)
-  )
-= let s = cbor_det_serialize x in
-  cbor_det_serialize_parse x;
-  cbor_det_parse_prefix s (s `Seq.append` y)
-
-let cbor_det_serialize_inj_strong
-  (x1 x2: cbor)
-  (y1 y2: Seq.seq U8.t)
-: Lemma
-  (requires (cbor_det_serialize x1 `Seq.append` y1 == cbor_det_serialize x2 `Seq.append` y2))
-  (ensures (x1 == x2 /\ y1 == y2))
-= cbor_det_serialize_parse' x1 y1;
-  cbor_det_serialize_parse' x2 y2;
-  Seq.lemma_append_inj
-    (cbor_det_serialize x1)
-    y1
-    (cbor_det_serialize x2)
-    y2
-
-let cbor_det_serialize_inj
-  (x1 x2: cbor)
-: Lemma
-  (requires (cbor_det_serialize x1 == cbor_det_serialize x2))
-  (ensures (x1 == x2))
-= Seq.append_empty_r (cbor_det_serialize x1);
-  Seq.append_empty_r (cbor_det_serialize x2);
-  cbor_det_serialize_inj_strong x1 x2 Seq.empty Seq.empty
